good

CXLMEM6.thy
@@ -1,141 +1,146 @@
-theory CXLMEM6 imports Main 
+theory CXLMEM6
+  imports Main
 begin
 
 (* Executable, order-agnostic next-state enumerators by flat-mapping over list elements *)
-(*how about using a third list for completed memory ops, and just prepend to that list, not involving 
-very complicated non-linear patterns on both the response channels and the mress list. (now doing)
-or even simpler, do not record the pending results in mress, just record every completed transaction with txid in mress. (implement in the future)
-even simpler is to use registers to hold read results, not keeping any issued/completed reads/writes. (implement in the future)
- 
-.*)
-definition m0 :: "nat \<Rightarrow> int" where
+(* how about using a third list for completed memory ops, and just prepend to that list, not involving
+   very complicated non-linear patterns on both the response channels and the mress list. (now doing, using a mapping instead of a list to avoid having to find the pended result with same txid)
+   or, even simpler, do not record the pending results in mress, just record every completed transaction with txid in mress. (implement in the future)
+   even simpler is to use registers to hold read results, not keeping any issued/completed reads/writes. (implement in the future) *)
+
+definition m0 :: "nat ⇒ int" where
   "m0 _ = 0"
 
 type_synonym txid = nat
-type_synonym mem = "nat \<Rightarrow> int"
+type_synonym mem = "nat ⇒ int"
 
 datatype Memop = Read nat | Write nat int
-
 datatype Memop_res = RdRes txid nat int | WrRes txid nat int | Pending txid Memop | NoEntry
 
-fun perform_Memop :: "Memop \<Rightarrow> (nat \<Rightarrow> int) \<Rightarrow> ((nat \<Rightarrow> int) * int)" where
+fun perform_Memop :: "Memop ⇒ (nat ⇒ int) ⇒ ((nat ⇒ int) * int)" where
   "perform_Memop (Read i) m = (m, m i)"
-| "perform_Memop (Write i v) m = (m ( i := v ), v)"
+| "perform_Memop (Write i v) m = (m (i := v), v)"
 
 datatype Req = MemRd txid nat
-
 datatype DRS = MemData txid int | MemData_NXM txid
-
 datatype Rwd = MemWrite txid nat int
-
 datatype NDR = Cmp txid | BI_ConflictAck txid
 
-datatype mem_msg = ReqMsg Req | RwdMsg Rwd | BIRsp | NDRMsg NDR | DRSMsg DRS  | BISnp
+datatype mem_msg = ReqMsg Req | RwdMsg Rwd | BIRsp | NDRMsg NDR | DRSMsg DRS | BISnp
 
-fun get_op_addr :: "mem_msg \<Rightarrow> nat" where
-  "get_op_addr m = (case m of (ReqMsg (MemRd txk i)) \<Rightarrow> i | _ \<Rightarrow> 0)"
+fun get_op_addr :: "mem_msg ⇒ nat" where
+  "get_op_addr m = (case m of ReqMsg (MemRd txk i) ⇒ i | _ ⇒ 0)"
 
-type_synonym regs = "nat \<Rightarrow> int"
+type_synonym regs = "nat ⇒ int"
 
 record cxl_state =
-  memory :: "nat \<Rightarrow> int"                  
-  m2sreqs :: "Req list"      
+  memory :: "nat ⇒ int"
+  m2sreqs :: "Req list"
   m2srwds :: "Rwd list"
   s2mdrss :: "DRS list"
   s2mndrs :: "NDR list"
   counter :: nat
-type_synonym state = "mem * Req list * Rwd list * DRS list * NDR list * nat * Memop list * (txid \<Rightarrow> Memop_res)"
-type_synonym state2 = "mem * Req list * Rwd list * DRS list * NDR list * nat * Memop list * regs"
-(*
-  input_events :: "Memop list"
-  output_events:: "Memop_completed list"
-  cxl_state: memory * m2sreqs * m2srwds * s2mdrss * counter
-*)
 
-fun flatmap :: "('a \<Rightarrow> 'b list) \<Rightarrow> 'a list \<Rightarrow> 'b list" where
-    "flatmap f [] = []"
-  | "flatmap f (x # xs) = f x @ flatmap f xs"
+type_synonym state =
+  "mem * Req list * Rwd list * DRS list * NDR list * nat * Memop list * (txid ⇒ Memop_res)"
+type_synonym state2 =
+  "mem * Req list * Rwd list * DRS list * NDR list * nat * Memop list * regs"
 
-fun enum_ctx :: "'a list \<Rightarrow> ('a list * 'a * 'a list) list" where
+(* generic helpers *)
+fun flatmap :: "('a ⇒ 'b list) ⇒ 'a list ⇒ 'b list" where
+  "flatmap f [] = []"
+| "flatmap f (x # xs) = f x @ flatmap f xs"
+
+fun enum_ctx :: "'a list ⇒ ('a list * 'a * 'a list) list" where
   "enum_ctx [] = []"
-| "enum_ctx (x#xs) = ([], x, xs) # map (\<lambda>(pre,y,suf). (x#pre, y, suf)) (enum_ctx xs)"
+| "enum_ctx (x#xs) = ([], x, xs) # map (λ(pre,y,suf). (x#pre, y, suf)) (enum_ctx xs)"
 
-(* flat_map helper *)
-fun flat_map :: "('a \<Rightarrow> 'b list) \<Rightarrow> 'a list \<Rightarrow> 'b list" where
+(* duplicated helper retained because later code uses this name *)
+fun flat_map :: "('a ⇒ 'b list) ⇒ 'a list ⇒ 'b list" where
   "flat_map f [] = []"
 | "flat_map f (x#xs) = f x @ flat_map f xs"
 
 (* External steps: combine four kinds of transitions *)
-fun external_nexts1 :: "state \<Rightarrow> state list" where
+fun external_nexts1 :: "state ⇒ state list" where
   "external_nexts1 (m, reqs, rwds, drss, ndrs, cnt, Read i # mops, mress) =
-      [(m, MemRd cnt i # reqs, rwds, drss, ndrs, cnt+1, mops, mress ( cnt := Pending cnt (Read i)))]"
+      [(m, MemRd cnt i # reqs, rwds, drss, ndrs, cnt+1, mops, mress (cnt := Pending cnt (Read i)))]"
 | "external_nexts1 (m, reqs, rwds, drss, ndrs, cnt, Write i v # mops, mress) =
       [(m, reqs, MemWrite cnt i v # rwds, drss, ndrs, cnt+1, mops, mress (cnt := Pending cnt (Write i v)))]"
 | "external_nexts1 _ = []"
 
-fun external_nexts2 :: "state \<Rightarrow> state list" where
+fun external_nexts2 :: "state ⇒ state list" where
 "external_nexts2 (m, reqs, rwds, drss, ndrs, cnt, mops, mress) = (
       let cmp_choices = enum_ctx ndrs;
-          wr_compl = flat_map (\<lambda>(pre1,x1,suf1).
-                        case x1 of Cmp tx \<Rightarrow>
-                            (case mress tx of Pending tx (Write i v) \<Rightarrow>
-                               [(m, reqs, rwds, drss, pre1 @ suf1, cnt, mops, mress (tx := WrRes tx i v)) ] | _ \<Rightarrow> [])
-                        | _ \<Rightarrow> [])  cmp_choices;
+          wr_compl = flat_map (λ(pre1,x1,suf1).
+                        case x1 of Cmp tx ⇒
+                          (case mress tx of Pending tx (Write i v) ⇒
+                               [(m, reqs, rwds, drss, pre1 @ suf1, cnt, mops, mress (tx := WrRes tx i v))] | _ ⇒ [])
+                        | _ ⇒ []) cmp_choices;
           drs_choices = enum_ctx drss;
-          rd_compl = flat_map (\<lambda>(pre1,x1,suf1).
-                        case x1 of MemData tx v \<Rightarrow>
-                            (case mress tx of Pending tx (Read i) \<Rightarrow>
-                               [(m, reqs, rwds, pre1 @ suf1, ndrs, cnt, mops, mress (tx := RdRes tx i v)) ] | _ \<Rightarrow> [])
-                          | _ \<Rightarrow> []) drs_choices
+          rd_compl = flat_map (λ(pre1,x1,suf1).
+                        case x1 of MemData tx v ⇒
+                          (case mress tx of Pending tx (Read i) ⇒
+                               [(m, reqs, rwds, pre1 @ suf1, ndrs, cnt, mops, mress (tx := RdRes tx i v))] | _ ⇒ [])
+                        | _ ⇒ []) drs_choices
       in wr_compl @ rd_compl)"
 
-fun external_nexts :: "state \<Rightarrow> state list" where
+fun external_nexts :: "state ⇒ state list" where
   "external_nexts s = external_nexts1 s @ external_nexts2 s"
 
-inductive  external_step :: "((nat => int) * Req list * Rwd list * DRS list * NDR list * nat * Memop list * Memop_res list)  => ((nat => int) * Req list * Rwd list * DRS list * NDR list * nat * Memop list * Memop_res list) \<Rightarrow> bool"
-  (infix "\<leadsto>e" 50)
-  where 
-    "(m, reqs, rwds, drss, ndrs, cnt, Read i # mops, mress) \<leadsto>e (m, MemRd cnt i # reqs, rwds, drss, ndrs, cnt+1, mops, Pending cnt (Read i) # mress)"
-  | "(m, reqs, rwds, drss, ndrs, cnt, Write i v # mops, mress) \<leadsto>e (m, reqs, MemWrite cnt i v # rwds, drss, ndrs, cnt+1, mops, Pending cnt (Write i v) # mress)"
-  | "(m, reqs, rwds, drss, ndrs1 @ [Cmp txid] @ ndrs2, cnt, mops, mress) \<leadsto>e (m, reqs, rwds, drss, ndrs1@ndrs2, cnt, mops, WrRes txid i v # mress)"
-  | "(m, reqs, rwds, drss1 @ [MemData txid v] @ drss2, ndrss, cnt, mops, mress) \<leadsto>e (m, reqs, rwds, drss1 @ drss2, ndrss, cnt, mops, RdRes txid i v # mress)"
+inductive  external_step ::
+  "((nat ⇒ int) * Req list * Rwd list * DRS list * NDR list * nat * Memop list * Memop_res list)
+    ⇒ ((nat ⇒ int) * Req list * Rwd list * DRS list * NDR list * nat * Memop list * Memop_res list) ⇒ bool"
+  (infix "⟶e" 50)
+where
+    "(m, reqs, rwds, drss, ndrs, cnt, Read i # mops, mress) ⟶e
+     (m, MemRd cnt i # reqs, rwds, drss, ndrs, cnt+1, mops, Pending cnt (Read i) # mress)"
+  | "(m, reqs, rwds, drss, ndrs, cnt, Write i v # mops, mress) ⟶e
+     (m, reqs, MemWrite cnt i v # rwds, drss, ndrs, cnt+1, mops, Pending cnt (Write i v) # mress)"
+  | "(m, reqs, rwds, drss, ndrs1 @ [Cmp txid] @ ndrs2, cnt, mops, mress) ⟶e
+     (m, reqs, rwds, drss, ndrs1@ndrs2, cnt, mops, WrRes txid i v # mress)"
+  | "(m, reqs, rwds, drss1 @ [MemData txid v] @ drss2, ndrss, cnt, mops, mress) ⟶e
+     (m, reqs, rwds, drss1 @ drss2, ndrss, cnt, mops, RdRes txid i v # mress)"
 
-
-fun internal_nexts :: "state \<Rightarrow> state list" where
+fun internal_nexts :: "state ⇒ state list" where
 "internal_nexts (m, reqs, rwds, drss, ndrs, cnt, mops, mress) = (
       let req_choices = enum_ctx reqs;
-          req_resp = flat_map (\<lambda>(pre1, x1, suf1).
-                        case x1 of MemRd tx i \<Rightarrow> [(m, pre1 @ suf1, rwds, MemData tx (m i) # drss, ndrs, cnt, mops, mress)]) req_choices;
+          req_resp = flat_map (λ(pre1, x1, suf1).
+                        case x1 of MemRd tx i ⇒
+                          [(m, pre1 @ suf1, rwds, MemData tx (m i) # drss, ndrs, cnt, mops, mress)]) req_choices;
           rwd_choices = enum_ctx rwds;
-          rwd_resp = flat_map (\<lambda>(pre1, x1, suf1).
-                        case x1 of MemWrite tx i v \<Rightarrow> [(m(i := v), reqs, pre1 @ suf1, drss, Cmp tx # ndrs, cnt, mops, mress)]) rwd_choices
+          rwd_resp = flat_map (λ(pre1, x1, suf1).
+                        case x1 of MemWrite tx i v ⇒
+                          [(m(i := v), reqs, pre1 @ suf1, drss, Cmp tx # ndrs, cnt, mops, mress)]) rwd_choices
       in req_resp @ rwd_resp)"
 
+inductive internal_step ::
+  "((nat ⇒ int) * Req list * Rwd list * DRS list * NDR list * nat * Memop list * Memop_res list)
+    ⇒ ((nat ⇒ int) * Req list * Rwd list * DRS list * NDR list * nat * Memop list * Memop_res list) ⇒ bool"
+  (infix "⟶i" 50)
+where
+    "(m, reqs1 @ [MemRd txid i] @ reqs2, rwds, drss, ndrs, cnt, mops, mress) ⟶i
+     (m, reqs1 @ reqs2, rwds, MemData txid (m i) # drss, ndrs, cnt, mops, mress)"
+  | "(m, reqs, rwds1 @ [MemWrite txid i v] @ rwds2, drss, ndrs, cnt, mops, mress) ⟶i
+     (m(i := v), reqs, rwds1 @ rwds2, drss, Cmp txid # ndrs, cnt, mops, mress)"
 
-inductive internal_step :: "((nat => int) * Req list * Rwd list * DRS list * NDR list * nat * Memop list * Memop_res list)  => ((nat => int) * Req list * Rwd list * DRS list * NDR list * nat * Memop list * Memop_res list) \<Rightarrow> bool"
-  (infix "\<leadsto>i" 50)
-  where
-    "(m, reqs1 @ [MemRd txid i] @ reqs2, rwds, drss, ndrs, cnt, mops, mress) \<leadsto>i (m, reqs1 @ reqs2, rwds, MemData txid (m i) # drss, ndrs, cnt, mops, mress)"
-  | "(m, reqs, rwds1 @ [MemWrite txid i v] @ rwds2, drss, ndrs, cnt, mops, mress) \<leadsto>i (m(i := v), reqs, rwds1 @ rwds2, drss, Cmp txid # ndrs, cnt, mops, mress)"
+inductive system_step ::
+  "((nat ⇒ int) * Req list * Rwd list * DRS list * NDR list * nat * Memop list * Memop_res list)
+    ⇒ ((nat ⇒ int) * Req list * Rwd list * DRS list * NDR list * nat * Memop list * Memop_res list) ⇒ bool"
+  (infix "⟶" 50)
+where
+    "tuple1 ⟶e tuple2 ⟹ tuple1 ⟶ tuple2"
+  | "tuple1 ⟶i tuple2 ⟹ tuple1 ⟶ tuple2"
 
-inductive system_step :: "((nat => int) * Req list * Rwd list * DRS list * NDR list * nat * Memop list * Memop_res list)  => ((nat => int) * Req list * Rwd list * DRS list * NDR list * nat * Memop list * Memop_res list) \<Rightarrow> bool"
-  (infix "\<leadsto>" 50)
-  where
-    "tuple1 \<leadsto>e tuple2 \<Longrightarrow> tuple1 \<leadsto> tuple2"
-  | "tuple1 \<leadsto>i tuple2 \<Longrightarrow> tuple1 \<leadsto> tuple2"
-
-definition system_nexts :: "state \<Rightarrow> state list"
-  where
+definition system_nexts :: "state ⇒ state list" where
   "system_nexts s = internal_nexts s @ external_nexts s"
 
 (* Example initial state *)
 definition mem3_42 :: "mem" where "mem3_42 = m0 (3 := 42)"
-
 definition initial1 :: state where
-  "initial1 = (mem3_42, [], [], [], [], 15, [Read 3], (\<lambda>tx. NoEntry))"
+  "initial1 = (mem3_42, [], [], [], [], 15, [Read 3], (λtx. NoEntry))"
 
 declare [[values_timeout = 5]]
-      
+
 value "external_nexts initial1"
 value "system_nexts initial1"
 
@@ -147,13 +152,10 @@ fun eval_until_end :: "nat ⇒ state ⇒ state list" where
        if ns = [] then [s] else concat (map (eval_until_end k) ns))"
 
 (* Examples *)
-
 value "eval_until_end 0 initial1"
 value "eval_until_end 1 initial1"
 value "eval_until_end 2 initial1"
 value "eval_until_end 3 initial1"
-
-
 value "eval_until_end 4 initial1"
 value "eval_until_end 5 initial1"
 
@@ -183,19 +185,18 @@ fun eval_until_end_ress :: "nat ⇒ state ⇒ (nat * Memop_res) list list" where
 (* Example *)
 value "eval_until_end_ress 3 initial1"
 
-(* CoRR (Coherent Read-Read) litmus: R(x); R(x) should not see newer then older.
-   Construct a scenario where first read can complete with a newer value (via drss),
+(* CoRR (Coherent Read-Read) litmus: R(x); R(x) should not observe “new then old”.
+   Construct a scenario where the first read can complete with a newer value (via drss),
    while memory still holds the old value, so the second read can observe the old one. *)
 definition LT_CORR :: state where
-  "LT_CORR = (m0, [], [], [], [], 0, [Read 3,Write 3 56, Read 3], (\<lambda>tx. NoEntry))"
+  "LT_CORR = (m0, [], [], [], [], 0, [Read 3, Write 3 56, Read 3], (λtx. NoEntry))"
 
 (* Explore only result mappings *)
 value "eval_until_end_ress 6 LT_CORR"
 
 (* Single-core litmus helpers and examples *)
-
 definition mem_set :: "(nat ⇒ int) ⇒ (nat * int) list ⇒ (nat ⇒ int)" where
-  "mem_set m xs = fold (λ(iv) f. f (fst iv := snd iv)) xs m"
+  "mem_set m xs = fold (λiv f. f (fst iv := snd iv)) xs m"
 
 definition mem_init :: "(nat * int) list ⇒ (nat ⇒ int)" where
   "mem_init xs = mem_set m0 xs"
@@ -203,25 +204,19 @@ definition mem_init :: "(nat * int) list ⇒ (nat ⇒ int)" where
 definition mk_state :: "(nat * int) list ⇒ nat ⇒ Memop list ⇒ state" where
   "mk_state inits cnt mops = (mem_init inits, [], [], [], [], cnt, mops, (λtx. NoEntry))"
 
-(* Litmus tests (single-core) *)
-
-(* RR: two reads observe the same memory *)
+(* Litmus tests (single core) *)
 definition LT_RR :: state where
   "LT_RR = mk_state [(3,42)] 0 [Read 3, Read 3]"
 
-(* WW: two writes recorded in order (memory not updated in this variant) *)
 definition LT_WW :: state where
   "LT_WW = mk_state [] 0 [Write 3 1, Write 3 2]"
 
-(* WR (same addr): read-after-write — with current model (no mem update), read observes old value *)
 definition LT_WR_same :: state where
   "LT_WR_same = mk_state [(3,0)] 0 [Write 3 1, Read 3]"
 
-(* WR (diff addr): read to another address unaffected *)
 definition LT_WR_diff :: state where
   "LT_WR_diff = mk_state [(3,0),(4,42)] 0 [Write 3 1, Read 4]"
 
-(* RW: read then write — read must observe the old value by program order *)
 definition LT_RW :: state where
   "LT_RW = mk_state [(5,7)] 0 [Read 5, Write 5 9]"
 
@@ -232,7 +227,7 @@ value "eval_until_end_ress 5 LT_WR_same"
 value "eval_until_end_ress 5 LT_WR_diff"
 value "eval_until_end_ress 5 LT_RW"
 
-(* ------ Dedup helpers (remove duplicates) ------ *)
+(* ------ De-dup helpers (remove duplicates) ------ *)
 
 (* For ress-only output, element type is (nat * Memop_res) list, which has executable equality *)
 definition eval_until_end_ress_nodup :: "nat ⇒ state ⇒ (nat * Memop_res) list list" where
@@ -264,26 +259,68 @@ value "eval_until_end_ress_nodup 6 LT_WR_diff"
 value "eval_until_end_ress_nodup 6 LT_RW"
 value "eval_until_end_keys_nodup 9 LT_CORR"
 
-(* ---------- Well-formedness: disallow orphan responses (no response without matching pending) ---------- *)
-fun wf_drss :: "DRS list ⇒ (txid ⇒ Memop_res) ⇒ bool" where
-  "wf_drss [] m = True"
-| "wf_drss (MemData tx _ # xs) m = (∃i. m tx = Pending tx (Read i)) ∧ wf_drss xs m"
-| "wf_drss (MemData_NXM tx # xs) m = (∃i. m tx = Pending tx (Read i)) ∧ wf_drss xs m"
+(* Read the memory value at address i from a state (helper: inspect terminal memory) *)
+fun mem_at :: "state ⇒ nat ⇒ int" where
+  "mem_at (m, _, _, _, _, _, _, _) i = m i"
 
-fun wf_ndrs :: "NDR list ⇒ (txid ⇒ Memop_res) ⇒ bool" where
-  "wf_ndrs [] m = True"
-| "wf_ndrs (Cmp tx # xs) m = (∃i v. m tx = Pending tx (Write i v)) ∧ wf_ndrs xs m"
-| "wf_ndrs (BI_ConflictAck _ # xs) m = wf_ndrs xs m"
+(* CoRR (Read; Read) — same thread reads the same address twice; should not observe “new then old” *)
+definition LT_CoRR_ok :: state where
+  "LT_CoRR_ok = mk_state [(3,42)] 0 [Read 3, Read 3]"
 
-fun wf_state :: "state ⇒ bool" where
-  "wf_state (m, reqs, rwds, drss, ndrs, cnt, mops, mress) = wf_drss drss mress ∧ wf_ndrs ndrs mress"
+(* CoRR-violation scenario (your LT_CORR is similar): R; W; R — if the first read can see the new value but the second read sees the old value, this violates CoRR *)
+definition LT_CoRR_bad :: state where
+  "LT_CoRR_bad = mk_state [] 0 [Read 3, Write 3 56, Read 3]"
 
-definition system_nexts_wf :: "state ⇒ state list" where
-  "system_nexts_wf s = filter wf_state (system_nexts s)"
+(* CoWR (same address): Write; Read — the read should at least see the value just written by the same thread *)
+definition LT_CoWR_same :: state where
+  "LT_CoWR_same = mk_state [(3,0)] 0 [Write 3 1, Read 3]"
 
-(* Examples (well-formed-only expansions) *)
-value "map mress_pairs (system_nexts_wf initial1)"
-value "map mress_pairs (filter wf_state (eval_until_end 3 initial1))"
+(* CoRW: Read; Write (same address) — the first read must not “see into the future” *)
+definition LT_CoRW1 :: state where
+  "LT_CoRW1 = mk_state [(3,7)] 0 [Read 3, Write 3 9]"
 
+(* CoRWR: Read; Write; Read (same address) — the two reads should be non-decreasing versions: cannot be “new then old” *)
+definition LT_CoRWR :: state where
+  "LT_CoRWR = mk_state [(3,0)] 0 [Read 3, Write 3 5, Read 3]"
+
+(* CoWW: Write; Write same address — later write should be ordered after earlier write globally (SC-per-location) *)
+definition LT_CoWW_same :: state where
+  "LT_CoWW_same = mk_state [(3,0)] 0 [Write 3 1, Write 3 2]"
+
+(* CoWW: different addresses — no strong ordering required *)
+definition LT_CoWW_diff :: state where
+  "LT_CoWW_diff = mk_state [(3,0),(4,100)] 0 [Write 3 1, Write 4 2]"
+
+(* Two address-independent sanity checks: WR/RW to different addresses *)
+definition LT_WR_diff2 :: state where
+  "LT_WR_diff2 = mk_state [(3,0),(4,42)] 0 [Write 3 1, Read 4]"
+
+definition LT_RW_diff2 :: state where
+  "LT_RW_diff2 = mk_state [(3,7),(4,11)] 0 [Read 3, Write 4 9]"
+
+declare [[values_timeout = 5]]
+
+(* CoRR normal case: both reads should be 42 *)
+value "eval_until_end_ress_nodup 6 LT_CoRR_ok"
+
+(* CoRR violation case: it may produce result pairs that are [new then old] *)
+value "eval_until_end_ress_nodup 7 LT_CoRR_bad"
+
+(* CoWR (same address): the read should at least see 1; the current model may still show 0 — indicates a possible CoWR violation *)
+value "eval_until_end_ress_nodup 7 LT_CoWR_same"
+
+(* CoRW: the first read should be the old value 7 *)
+value "eval_until_end_ress_nodup 7 LT_CoRW1"
+
+(* CoRWR: pairs of the two read results — check whether (r1=5, r2=0) (new then old) can occur *)
+value "eval_until_end_ress_nodup 8 LT_CoRWR"
+
+(* CoWW end-state memory cell 3 value set; if {1,2} is a subset of this set, write–write reordering is possible for the same address *)
+value "remdups (map (λs. mem_at s 3) (eval_until_end 8 LT_CoWW_same))"
+
+(* CoWW (different addresses) and WR/RW (different addresses) as a comparison *)
+value "eval_until_end_ress_nodup 6 LT_CoWW_diff"
+value "eval_until_end_ress_nodup 6 LT_WR_diff2"
+value "eval_until_end_ress_nodup 6 LT_RW_diff2"
 
 end
